Grounding_Pipeline.thy
@@ -1,0 +1,139 @@
+theory Grounding_Pipeline
+imports Type_Normalization Goal_Normalization Precondition_Normalization
+begin
+
+subsection \<open> Setting up compact notations \<close>
+
+context ast_problem begin
+thm detype_prob_sel
+thm ast_problem2.prob_detyped
+lemma detype_prob_wf_compact:
+  "restrict_prob \<Longrightarrow> wf_problem
+  \<Longrightarrow> ast_problem.wf_problem detype_prob"
+  using restr_problem2.detype_prob_wf
+  using restr_problem2.intro restr_problem.intro restr_problem_axioms.intro wf_ast_problem.intro
+  by auto
+lemma detyped_valid_iff_compact:
+  "restrict_prob \<Longrightarrow> wf_problem
+  \<Longrightarrow> valid_plan \<pi>s \<longleftrightarrow> ast_problem.valid_plan (detype_prob) \<pi>s"
+  using restr_problem2.detyped_valid_iff
+  using restr_problem2.intro restr_problem.intro restr_problem_axioms.intro wf_ast_problem.intro
+  by auto
+
+thm ast_problem.degoal_prob_sel
+lemma degoal_prob_wf_compact:
+  "wf_problem \<Longrightarrow> ast_problem.wf_problem (degoal_prob)"
+  using wf_ast_problem3.degoal_prob_wf
+  using wf_ast_problem3_def wf_ast_problem.intro by simp
+lemma degoal_plan_restore_compact:
+  "wf_problem \<Longrightarrow> ast_problem.valid_plan degoal_prob \<pi>s \<Longrightarrow> valid_plan (restore_plan_degoal \<pi>s)"
+  using wf_ast_problem3.valid_plan_left
+  using wf_ast_problem3_def wf_ast_problem.intro by simp
+lemma degoaled_valid_iff_compact:
+  "wf_problem \<Longrightarrow> (\<exists>\<pi>s. valid_plan \<pi>s) = (\<exists>\<pi>s'. ast_problem.valid_plan degoal_prob \<pi>s')"
+  using wf_ast_problem3.degoaled_valid_iff
+  using wf_ast_problem3_def wf_ast_problem.intro by simp
+
+thm ast_problem.split_prob_sel
+thm ast_problem4.prec_normed_prob
+lemma split_prob_wf_compact:
+  "wf_problem \<Longrightarrow> ast_problem.wf_problem (split_prob)"
+  using wf_ast_problem4.split_prob_wf
+  using wf_ast_problem4_def wf_ast_problem.intro by simp
+lemma split_valid_iff_compact:
+  "wf_problem \<Longrightarrow> (\<exists>\<pi>s. valid_plan \<pi>s) = (\<exists>\<pi>s'. ast_problem.valid_plan split_prob \<pi>s')"
+  using wf_ast_problem4.split_valid_iff
+  using wf_ast_problem4_def wf_ast_problem.intro by simp
+lemma restore_plan_split_valid_compact:
+  "wf_problem \<Longrightarrow> ast_problem.valid_plan split_prob \<pi>s \<Longrightarrow> valid_plan (restore_plan_split \<pi>s)"
+  using wf_ast_problem4.restore_plan_split_valid
+  using wf_ast_problem4_def wf_ast_problem.intro by simp
+
+end
+
+subsection \<open> Normalization correctness \<close>
+
+context ast_problem begin
+
+definition "P\<^sub>N \<equiv> ast_problem.split_prob (ast_problem.degoal_prob detype_prob)"
+
+definition "normalized_prob \<equiv>
+  typeless_prob \<and> (is_conj (goal P)) \<and> prec_normed_prob"
+
+definition "reconstruct_plan_norm \<pi>s \<equiv>
+  ast_domain.restore_plan_degoal detype_dom
+    (ast_domain.restore_plan_split (ast_problem.degoal_dom detype_prob) \<pi>s)"
+
+text \<open> goal and precondition normalization preserve type normalization \<close>
+lemma goal_norm_preserves_typeless:
+  "typeless_prob \<Longrightarrow> ast_problem.typeless_prob (degoal_prob)"
+  unfolding ast_problem.typeless_prob_def ast_domain.typeless_dom_def
+    degoal_prob_sel degoal_dom_sel
+  unfolding goal_pred_decl_def goal_ac_def by auto
+
+lemma prec_norm_preserves_typeless:
+  "typeless_prob \<Longrightarrow> ast_problem.typeless_prob (split_prob)"
+  unfolding ast_problem.typeless_prob_def ast_domain.typeless_dom_def
+    split_prob_sel split_dom_sel
+  unfolding split_acs_def using split_ac_sel(2) by auto
+
+text \<open> type and precondition normalization preserve goal normalization \<close>
+lemma type_norm_preserves_goal_conj:
+  "is_conj (goal P) \<Longrightarrow> is_conj (goal detype_prob)"
+  unfolding detype_prob_sel .
+
+lemma prec_norm_preserves_goal_conj:
+  "is_conj (goal P) \<Longrightarrow> is_conj (goal split_prob)"
+  unfolding split_prob_sel .
+
+text \<open> Due to my implementation of is_conj and type-normed action preconditions,
+  type normalization does not preserve precondition normalization.
+  E.g: (is_Car (x) \<and> is_Road (y)) \<and> (at (x, z) \<and> at (w, z)) is not a right deep tree. \<close>
+(* TODO use conjAnd in type normalization*)
+
+text \<open> Goal normalization only preserves precondition normalization if the goal is a
+  pure conjunction.\<close>
+
+lemma goal_norm_preserves_prec_norm:
+  assumes "prec_normed_prob"
+    "is_conj (goal P)"
+  shows "ast_problem.prec_normed_prob degoal_prob"
+  using assms(1) unfolding ast_domain.prec_normed_dom_def
+  unfolding degoal_prob_sel degoal_dom_sel
+  unfolding goal_ac_def term_goal_def
+  using map_preserves_isconj assms(2) by auto
+
+theorem normalization_normalizes:
+  "ast_problem.normalized_prob P\<^sub>N"
+  unfolding ast_problem.normalized_prob_def P\<^sub>N_def
+  using ast_problem2.prob_detyped
+  using ast_problem.degoal_prob_sel(4) ast_problem.goal_norm_preserves_typeless
+  using ast_problem.prec_norm_preserves_typeless ast_problem.prec_norm_preserves_goal_conj
+    ast_problem4.prec_normed_prob by simp
+
+theorem normalization_wf:
+  "restrict_prob \<Longrightarrow> wf_problem \<Longrightarrow> ast_problem.wf_problem P\<^sub>N"
+  unfolding P\<^sub>N_def
+  using detype_prob_wf_compact ast_problem.degoal_prob_wf_compact ast_problem.split_prob_wf_compact
+  by simp
+
+theorem normalization_valid_iff:
+  "restrict_prob \<Longrightarrow> wf_problem \<Longrightarrow>
+    (\<exists>\<pi>s. valid_plan \<pi>s) \<longleftrightarrow> (\<exists>\<pi>s'. ast_problem.valid_plan P\<^sub>N \<pi>s')"
+  unfolding P\<^sub>N_def
+  using detype_prob_wf_compact ast_problem.degoal_prob_wf_compact
+  using detyped_valid_iff_compact ast_problem.degoaled_valid_iff_compact
+    ast_problem.split_valid_iff_compact by simp
+
+theorem normalization_reconstruct:
+  "restrict_prob \<Longrightarrow> wf_problem \<Longrightarrow>
+    ast_problem.valid_plan P\<^sub>N \<pi>s \<Longrightarrow> valid_plan (reconstruct_plan_norm \<pi>s)"
+  unfolding P\<^sub>N_def reconstruct_plan_norm_def
+  using detype_prob_wf_compact ast_problem.degoal_prob_wf_compact
+  using ast_problem.restore_plan_split_valid_compact ast_problem.degoal_plan_restore_compact
+    detyped_valid_iff_compact
+  by (metis ast_problem.degoal_prob_sel(1) detype_prob_sel(1))
+
+end
+
+end
